add height as metadata 4/n: Impl.Trees.Rotate is done?
impossible to check on a 12G machine...

Impl.Trees.Rotate.fst
@@ -78,15 +78,21 @@ let rotate_left (#a: Type) (ptr: t a)
 //#push-options "--ifuel 1 --fuel 2"
 
 //@Trees (rotate*)
-#push-options "--fuel 1 --ifuel 1"
+#push-options "--fuel 1 --ifuel 1 --z3rlimit 25"
 let rotate_left (#a: Type) (ptr: t a)
   : Steel (t a)
   (linked_tree ptr)
   (fun ptr' -> linked_tree ptr')
   (requires (fun h0 ->
-    Some? (Spec.rotate_left_wds (v_linked_tree ptr h0))))
+    let t = v_linked_tree ptr h0 in
+    let r = Spec.rotate_left_wdm t in
+    Some? r /\
+    Spec.height_of_tree (Spec.get r) <= Spec.height_of_tree t
+  ))
+
   (ensures (fun h0 ptr' h1 ->
-    Spec.rotate_left_wds (v_linked_tree ptr h0) == Some (v_linked_tree ptr' h1)
+    Spec.rotate_left_wdm (v_linked_tree ptr h0)
+    == Some (v_linked_tree ptr' h1)
   ))
   =
   let h = get () in
@@ -100,26 +106,44 @@ let rotate_left (#a: Type) (ptr: t a)
   let z = get_data z_node in
   let s1 = sot_wds (get_left x_node) in
   let s2 = sot_wds (get_left z_node) in
-  let sx = U.add (U.add s1 s2) one in
-  write (get_size z_node) sx;
-  let new_subnode = mk_node x (get_left x_node) (get_left z_node) (get_size z_node) in
-  let new_node = mk_node z ptr (get_right z_node) (get_size x_node) in
+  let s12 = U.add (U.add s1 s2) one in
+
+  let h1 = hot_wdh (get_left x_node) in
+  let h2 = hot_wdh (get_left z_node) in
+  let h3 = hot_wdh (get_right z_node) in
+  let h12 = if U.gt h1 h2 then U.add h1 one else U.add h2 one in
+  let h123 = if U.gt h12 h3 then U.add h12 one else U.add h3 one in
+  write (get_size z_node) s12;
+  write (get_height z_node) h12;
+  let new_subnode = mk_node x
+    (get_left x_node) (get_left z_node)
+    (get_size z_node) (get_height z_node) in
+  write (get_height x_node) h123;
+  let new_node = mk_node z ptr (get_right z_node)
+    (get_size x_node) (get_height x_node) in
   write (get_right x_node) new_node;
   write ptr new_subnode;
-  (**) pack_tree ptr (get_left x_node) (get_left z_node) (get_size z_node);
-  (**) pack_tree (get_right x_node) ptr (get_right z_node) (get_size x_node);
+  (**) pack_tree ptr (get_left x_node) (get_left z_node)
+  (get_size z_node) (get_height z_node);
+  (**) pack_tree (get_right x_node) ptr (get_right z_node)
+  (get_size x_node) (get_height x_node);
   return (get_right x_node)
 #pop-options
 
-#push-options "--fuel 1 --ifuel 1"
+#push-options "--fuel 1 --ifuel 1 --z3rlimit 25"
 let rotate_right (#a: Type) (ptr: t a)
   : Steel (t a)
   (linked_tree ptr)
   (fun ptr' -> linked_tree ptr')
   (requires (fun h0 ->
-    Some? (Spec.rotate_right_wds (v_linked_tree ptr h0))))
+    let t = v_linked_tree ptr h0 in
+    let r = Spec.rotate_right_wdm t in
+    Some? r /\
+    Spec.height_of_tree (Spec.get r) <= Spec.height_of_tree t
+  ))
   (ensures (fun h0 ptr' h1 ->
-    Spec.rotate_right_wds (v_linked_tree ptr h0) == Some (v_linked_tree ptr' h1)
+    Spec.rotate_right_wdm (v_linked_tree ptr h0)
+    == Some (v_linked_tree ptr' h1)
   ))
   =
   let h = get () in
@@ -133,32 +157,49 @@ let rotate_right (#a: Type) (ptr: t a)
   let z = get_data z_node in
   let s1 = sot_wds (get_right z_node) in
   let s2 = sot_wds (get_right x_node) in
-  let sx = U.add (U.add s1 s2) one in
-  write (get_size z_node) sx;
-  let new_subnode = mk_node x (get_right z_node) (get_right x_node) (get_size z_node) in
-  let new_node = mk_node z (get_left z_node) ptr (get_size x_node) in
+  let s12 = U.add (U.add s1 s2) one in
+
+  let h1 = hot_wdh (get_right z_node) in
+  let h2 = hot_wdh (get_right x_node) in
+  let h3 = hot_wdh (get_left z_node) in
+  let h12 = if U.gt h1 h2 then U.add h1 one else U.add h2 one in
+  let h123 = if U.gt h12 h3 then U.add h12 one else U.add h3 one in
+  write (get_size z_node) s12;
+  write (get_height z_node) h12;
+  let new_subnode = mk_node x (get_right z_node) (get_right x_node)
+    (get_size z_node) (get_height z_node) in
+  write (get_height x_node) h123;
+  let new_node = mk_node z (get_left z_node) ptr
+    (get_size x_node) (get_height x_node) in
   write (get_left x_node) new_node;
   write ptr new_subnode;
-  (**) pack_tree ptr (get_right z_node) (get_right x_node) (get_size z_node);
-  (**) pack_tree (get_left x_node) (get_left z_node) ptr (get_size x_node);
+  (**) pack_tree ptr (get_right z_node) (get_right x_node)
+    (get_size z_node) (get_height z_node);
+  (**) pack_tree (get_left x_node) (get_left z_node) ptr
+    (get_size x_node) (get_height x_node);
   return (get_left x_node)
 #pop-options
 
-#push-options "--fuel 1 --ifuel 1"
+#push-options "--fuel 1 --ifuel 1 --z3rlimit 50"
 let rotate_right_left (#a: Type) (ptr: t a)
   : Steel (t a)
   (linked_tree ptr)
   (fun ptr' -> linked_tree ptr')
   (requires (fun h0 ->
-    Some? (Spec.rotate_right_left_wds (v_linked_tree ptr h0))))
+    let t = v_linked_tree ptr h0 in
+    let r = Spec.rotate_right_left_wdm t in
+    Some? r /\
+    Spec.height_of_tree (Spec.get r) <= Spec.height_of_tree t
+  ))
   (ensures (fun h0 ptr' h1 ->
-    Spec.rotate_right_left_wds (v_linked_tree ptr h0) == Some (v_linked_tree ptr' h1)
+    Spec.rotate_right_left_wdm (v_linked_tree ptr h0)
+    == Some (v_linked_tree ptr' h1)
   ))
   =
   let h = get () in
   assert (Spec.size_of_tree (v_linked_tree ptr h) <= c);
   Spec.rotate_right_left_size (v_linked_tree ptr h);
-  assert (Spec.size_of_tree (Spec.get (Spec.rotate_right_left_wds (v_linked_tree ptr h)))
+  assert (Spec.size_of_tree (Spec.get (Spec.rotate_right_left_wdm (v_linked_tree ptr h)))
   == Spec.size_of_tree (v_linked_tree ptr h));
   (**) node_is_not_null ptr;
   // original root node
@@ -178,40 +219,63 @@ let rotate_right_left (#a: Type) (ptr: t a)
   let s2 = sot_wds (get_left y_node) in
   let s3 = sot_wds (get_right y_node) in
   let s4 = sot_wds (get_right z_node) in
-  let s12 = U.add (U.add s1 s2) one in
-  let s34 = U.add (U.add s3 s4) one in
-  write (get_size y_node) s12;
-  write (get_size z_node) s34;
 
-  let new_x = mk_node x (get_left x_node) (get_left y_node) (get_size y_node) in
-  let new_z = mk_node z (get_right y_node) (get_right z_node) (get_size z_node) in
-  let new_y = mk_node y ptr (get_right x_node) (get_size x_node) in
+  let h1 = hot_wdh (get_left x_node) in
+  let h2 = hot_wdh (get_left y_node) in
+  let h3 = hot_wdh (get_right y_node) in
+  let h4 = hot_wdh (get_right z_node) in
+  let h12 = if U.gt h1 h2 then U.add h1 one else U.add h2 one in
+  let h34 = if U.gt h3 h4 then U.add h3 one else U.add h4 one in
+  let h1234 = if U.gt h12 h34 then U.add h12 one else U.add h34 one in
+
+  let s12 = U.add (U.add s1 s2) one in
+  write (get_size y_node) s12;
+  write (get_height y_node) h12;
+  let s34 = U.add (U.add s3 s4) one in
+  write (get_size z_node) s34;
+  write (get_height z_node) h34;
+  write (get_height x_node) h1234;
+
+  let new_x = mk_node x (get_left x_node) (get_left y_node)
+    (get_size y_node) (get_height y_node) in
+  let new_z = mk_node z (get_right y_node) (get_right z_node)
+    (get_size z_node) (get_height z_node) in
+  let new_y = mk_node y ptr (get_right x_node)
+    (get_size x_node) (get_height x_node) in
 
   write ptr new_x;
   write (get_right x_node) new_z;
   write (get_left z_node) new_y;
 
-  (**) pack_tree ptr (get_left x_node) (get_left y_node) (get_size y_node);
-  (**) pack_tree (get_right x_node) (get_right y_node) (get_right z_node) (get_size z_node);
-  (**) pack_tree (get_left z_node) ptr (get_right x_node) (get_size x_node);
+  (**) pack_tree ptr (get_left x_node) (get_left y_node)
+    (get_size y_node) (get_height y_node);
+  (**) pack_tree (get_right x_node) (get_right y_node) (get_right z_node)
+    (get_size z_node) (get_height z_node);
+  (**) pack_tree (get_left z_node) ptr (get_right x_node)
+    (get_size x_node) (get_height x_node);
 
   return (get_left z_node)
 #pop-options
 
-#push-options "--fuel 1 --ifuel 1"
+#push-options "--fuel 1 --ifuel 1 --z3rlimit 50"
 let rotate_left_right (#a: Type) (ptr: t a)
   : Steel (t a)
   (linked_tree ptr)
   (fun ptr' -> linked_tree ptr')
-  (requires fun h0 -> Some? (Spec.rotate_left_right_wds (v_linked_tree ptr h0)))
+  (requires (fun h0 ->
+    let t = v_linked_tree ptr h0 in
+    let r = Spec.rotate_left_right_wdm t in
+    Some? r /\
+    Spec.height_of_tree (Spec.get r) <= Spec.height_of_tree t
+  ))
   (ensures (fun h0 ptr' h1 ->
-    Spec.rotate_left_right_wds (v_linked_tree ptr h0) == Some (v_linked_tree ptr' h1)
+    Spec.rotate_left_right_wdm (v_linked_tree ptr h0) == Some (v_linked_tree ptr' h1)
   ))
   =
   let h = get () in
   assert (Spec.size_of_tree (v_linked_tree ptr h) <= c);
   Spec.rotate_left_right_size (v_linked_tree ptr h);
-  assert (Spec.size_of_tree (Spec.get (Spec.rotate_left_right_wds (v_linked_tree ptr h)))
+  assert (Spec.size_of_tree (Spec.get (Spec.rotate_left_right_wdm (v_linked_tree ptr h)))
   == Spec.size_of_tree (v_linked_tree ptr h));
   (**) node_is_not_null ptr;
   // original root node
@@ -235,22 +299,41 @@ let rotate_left_right (#a: Type) (ptr: t a)
   let s2 = sot_wds (get_left y_node) in
   let s3 = sot_wds (get_right y_node) in
   let s4 = sot_wds (get_right x_node) in
-  let s12 = U.add (U.add s1 s2) one in
-  let s34 = U.add (U.add s3 s4) one in
-  write (get_size y_node) s12;
-  write (get_size z_node) s34;
 
-  let new_z = mk_node z (get_left z_node) (get_left y_node) (get_size y_node) in
-  let new_x = mk_node x (get_right y_node) (get_right x_node) (get_size z_node) in
-  let new_y = mk_node y (get_left x_node) ptr (get_size x_node) in
+
+  let h1 = hot_wdh (get_left z_node) in
+  let h2 = hot_wdh (get_left y_node) in
+  let h3 = hot_wdh (get_right y_node) in
+  let h4 = hot_wdh (get_right x_node) in
+  let h12 = if U.gt h1 h2 then U.add h1 one else U.add h2 one in
+  let h34 = if U.gt h3 h4 then U.add h3 one else U.add h4 one in
+  let h1234 = if U.gt h12 h34 then U.add h12 one else U.add h34 one in
+
+  let s12 = U.add (U.add s1 s2) one in
+  write (get_size y_node) s12;
+  write (get_height y_node) h12;
+  let s34 = U.add (U.add s3 s4) one in
+  write (get_size z_node) s34;
+  write (get_height z_node) h34;
+  write (get_height x_node) h1234;
+
+  let new_z = mk_node z (get_left z_node) (get_left y_node)
+    (get_size y_node) (get_height y_node) in
+  let new_x = mk_node x (get_right y_node) (get_right x_node)
+    (get_size z_node) (get_height z_node) in
+  let new_y = mk_node y (get_left x_node) ptr
+    (get_size x_node) (get_height x_node) in
 
   write (get_left x_node) new_z;
   write ptr new_x;
   write (get_right z_node) new_y;
 
-  (**) pack_tree (get_left x_node) (get_left z_node) (get_left y_node) (get_size y_node);
-  (**) pack_tree ptr (get_right y_node) (get_right x_node) (get_size z_node);
-  (**) pack_tree (get_right z_node) (get_left x_node) ptr (get_size x_node);
+  (**) pack_tree (get_left x_node) (get_left z_node) (get_left y_node)
+    (get_size y_node) (get_height y_node);
+  (**) pack_tree ptr (get_right y_node) (get_right x_node)
+    (get_size z_node) (get_height z_node);
+  (**) pack_tree (get_right z_node) (get_left x_node) ptr
+    (get_size x_node) (get_height x_node);
 
   return (get_right z_node)
 #pop-options
